eval: AEval, BEval, and two evaluation defs for Com

SoftwareFoundations2/Eval/Eval.lean
@@ -1,29 +1,7 @@
-import SoftwareFoundations2.Syntax
+import SoftwareFoundations2.Eval.State
 
-#check ⟨{ 2 + 3 }⟩
-
-/--
-    A `machine state` (or just `state`) represents the current values
-      of all variables at some point in the execution of a program.
-
-    For simplicity, we make the following assumptions:
-    - all variables are global;
-    - variables only hold numbers;
-    - the state is defined for _all_ variables, even though any given
-      program is only able to mention a finite number of them.
-
-    Because each variable stores a natural number, we can represent the state
-      as a function from `Strings` (variable names) to `Nat`, and will use `0` as
-      default value in the store.
--/
-def State : Type := String → Nat
-
-instance : Inhabited State where
-  default := λ _ => 0
-
-/--
-  Evaluating an arithmetic expression in a given state `σ` produces a number.
--/
+/-- Evaluating an arithmetic expression in a given state `σ` produces a number. -/
+@[simp]
 def AExp.eval (σ : State) : AExp → Nat
   | ANum n       => n
   | AId x        => σ x
@@ -31,9 +9,8 @@ def AExp.eval (σ : State) : AExp → Nat
   | AMinus a1 a2 => a1.eval σ - a2.eval σ
   | AMult a1 a2  => a1.eval σ * a2.eval σ
 
-/--
-  Evaluating a boolean expression in a given state `σ` produces a boolean.
--/
+/-- Evaluating a boolean expression in a given state `σ` produces a boolean. -/
+@[simp]
 def BExp.eval (σ : State) : BExp → Bool
   | BTrue      => true
   | BFalse     => false
@@ -43,3 +20,85 @@ def BExp.eval (σ : State) : BExp → Bool
   | BGt a1 a2  => a1.eval σ > a2.eval σ
   | BNot b     => !b.eval σ
   | BAnd b1 b2 => b1.eval σ && b2.eval σ
+
+/-- Evaluating a command in a given state `σ` produces a new state.
+
+    Note that this function is marked as `partial`.
+    This means that for some commands it is provided as input,
+    it may run forever and fail to return a final state.
+
+    (Consider, for example, the command `while btrue do skip od`. Try to execute
+    `Com.eval` on this command and see what happens.)
+
+    The issue is that, mathematically, functions must be **total**: they must map **every** value
+    in their domain to a definite value in their codomain.
+    Accordingly, in Lean, we can't use partial functions in proofs; they do not correspond to a
+    well-defined mathematical object.
+
+    We use the definition below only for debugging. It's basically a really simple interpreter for
+    IMP: pass in a command and an initial state, and it will execute the command and (if it
+    terminates) yield the final state. Feel free to play with it!
+
+    But to prove properties about IMP commands, we will provide a new definition shortly.
+    The new definition will be given as a *relation* between states, commands and states;
+    not as a *function*.
+-/
+partial def Com.eval (σ : State) : Com → State
+  | CSkip       => σ
+  | CAsgn x a   => σ[x ↦ a.eval σ]
+  | CSeq c1 c2  => (c2.eval ∘ c1.eval) σ
+  | CIf b c1 c2 => if b.eval σ then c1.eval σ else c2.eval σ
+  | CWhile b c  => if b.eval σ then ((CWhile b c).eval ∘ c.eval) σ else σ
+
+/-- Evaluates a command and prints computes the value of each program
+    variable in the final state `σ'`.
+-/
+def Com.getOutput (c : Com) (σ : State) : List (Var × Nat) :=
+  let σ' := c.eval σ
+  List.foldr (fun x acc => ⟨x, σ' x⟩ :: acc) [] c.vars
+
+-- An example:
+#eval ⟨{
+  sum = 0;
+  i = 0;
+  while (i <= n) do
+    sum = sum + i;
+    i = i + 1;
+  od
+}⟩.getOutput ["n" ↦ 7]
+
+open Com
+
+/-- Big-step evaluation relation. -/
+inductive ComEval : State → Com → State → Prop where
+  | ESkip :
+        ComEval σ CSkip σ
+  | EAsgn :
+        n = a.eval σ →
+        σ' = σ[x ↦ n] →
+          ComEval σ (CAsgn x a) σ'
+  | ESeq :
+        ComEval σ c₁ σ'   →
+        ComEval σ' c₂ σ'' →
+          ComEval σ (CSeq c₁ c₂) σ''
+  | EIfTrue :
+        b.eval σ = true →
+        ComEval σ c₁ σ' →
+          ComEval σ (CIf b c1 c2) σ'
+  | EIfFalse :
+        b.eval σ = false →
+        ComEval σ c₂ σ' →
+          ComEval σ (CIf b c₁ c₂) σ'
+  | EWhileFalse :
+        b.eval σ = false →
+          ComEval σ (CWhile b c) σ
+  | EWhileTrue :
+        b.eval σ = true →
+        ComEval σ c σ' →
+        ComEval σ' (CWhile b c) σ'' →
+          ComEval σ (CWhile b c) σ''
+
+notation σ:arg " =[" com "]=> " σ':arg => ComEval σ com σ'
+syntax term " =[" com "]=> " term : term
+macro_rules
+  | `($st1 =[ $com:com ]=> $st2) => `(ComEval $st1 ⟨{ $com:com }⟩ $st2)
