SoftwareFoundations2/Syntax/AST.lean
@@ -1,12 +1,17 @@
+import Mathlib.Data.List.Dedup
+
+abbrev Var : Type := String
+
 /-
   Abstract syntax of arithmetic expressions
 -/
 inductive AExp where
   | ANum   (n : Nat)
-  | AId    (x : String)
+  | AId    (x : Var)
   | APlus  (a1 a2 : AExp)
   | AMinus (a1 a2 : AExp)
   | AMult  (a1 a2 : AExp)
+deriving Repr
 
 /-
   Abstract syntax of boolean expressions
@@ -20,13 +25,41 @@ inductive BExp where
   | BGt    (a1 a2 : AExp)
   | BNot   (b : BExp)
   | BAnd   (b1 b2 : BExp)
+deriving Repr
 
 /-
   Abstract syntax of commands
 -/
 inductive Com where
   | CSkip
-  | CAsgn  (x : String) (a : AExp)
+  | CAsgn  (x : Var) (a : AExp)
   | CSeq   (c1 c2 : Com)
   | CIf    (b : BExp) (c1 c2 : Com)
   | CWhile (b : BExp) (c : Com)
+deriving Repr
+
+/- List of all variables occurring in an arithmetic expression -/
+def AExp.vars : AExp → List Var
+  | AId x        => [x]
+  | APlus a1 a2  => List.dedup <| a1.vars ++ a2.vars
+  | AMinus a1 a2 => List.dedup <| a1.vars ++ a2.vars
+  | AMult a1 a2  => List.dedup <| a1.vars ++ a2.vars
+  | _            => []
+
+/- List of all variables occurring in a boolean expression -/
+def BExp.vars : BExp → List Var
+  | BEq  a1 a2   => List.dedup <| a1.vars ++ a2.vars
+  | BNeq a1 a2   => List.dedup <| a1.vars ++ a2.vars
+  | BLe  a1 a2   => List.dedup <| a1.vars ++ a2.vars
+  | BGt a1 a2    => List.dedup <| a1.vars ++ a2.vars
+  | BNot b       => b.vars
+  | BAnd b1 b2   => List.dedup <| b1.vars ++ b2.vars
+  | _            => []
+
+/- List of all variables occurring in a command -/
+def Com.vars : Com → List Var
+  | CSkip       => []
+  | CAsgn x a   => List.dedup <| x :: a.vars
+  | CSeq c1 c2  => List.dedup <| c1.vars ++ c2.vars
+  | CIf b c1 c2 => List.dedup <| b.vars ++ c1.vars ++ c2.vars
+  | CWhile b c  => List.dedup <| b.vars ++ c.vars
