SoftwareFoundations2/Eval/Examples.lean
@@ -1,0 +1,32 @@
+import SoftwareFoundations2.Eval.Eval
+
+open ComEval
+
+theorem ceval_example1 :
+  σ =[
+      x = 2;
+      if (x <= 1) then
+        y = 3;
+      else
+        z = 4;
+      endif
+  ]=> σ["z" ↦ 4]["x" ↦ 2] := by
+  apply ESeq
+  · apply EAsgn
+    · rfl
+    · rfl
+  · apply EIfFalse
+    · rfl
+    · apply EAsgn
+      · rfl
+      · simp only [AExp.eval]
+        grind
+
+theorem ceval_example2 :
+  σ =[
+    x = 0;
+    y = 1;
+    z = 2
+  ]=> σ["z"↦2]["y"↦1]["x"↦0] := by
+  -- FILL IN HERE
+  sorry
