SoftwareFoundations2/Eval/State.lean
@@ -1,0 +1,33 @@
+import SoftwareFoundations2.Syntax
+
+/-- A `machine state` (or just `state`) represents the current values
+      of all variables at some point in the execution of a program.
+
+    For simplicity, we make the following assumptions:
+    - all variables are global;
+    - variables only hold numbers;
+    - the state is defined for _all_ variables, even though any given
+      program is only able to mention a finite number of them.
+
+    Because each variable stores a natural number, we can represent the state
+      as a function from `Var` (which is an alias for `String`; i.e., variable names)
+      to `Nat`, and will use `0` as default value in the store.
+-/
+def State : Type := Var → Nat
+
+instance : Inhabited State where
+  default := fun _ => 0
+
+def State.init : State := Inhabited.default
+def State.set (σ : State) (x : Var) (v : Nat) : State :=
+  fun x' => if x' == x then v else σ x'
+
+notation "·" => State.init
+notation "[" x " ↦ " v "]" => State.set State.init x v
+notation s "[" x " ↦ " v "]" => State.set s x v
+
+@[grind =]
+theorem State.set_comm {xn yn : Nat} (h : x ≠ y) : σ[x ↦ xn][y ↦ yn] = σ[y ↦ yn][x ↦ xn] := by
+  unfold State.set
+  funext str
+  grind
